Criando subst

src/Coq/Syntax.v
@@ -1,68 +1,107 @@
 Require Import List.
+Require Import SfLib.
 
-Notation Id := nat.
 Notation "'[' X ']'" := (list X) (at level 40).
 (* We will use Notation to make automation easier
  * This will be the notation to be similar with haskell *)
 
 Inductive ClassName :=
   | ClassObject : ClassName
-  | ClassId : Id -> ClassName.
+  | ClassId : id -> ClassName.
  
 Inductive Var :=
   | This : Var
-  | VarId: Id -> Var.
+  | VarId: id -> Var.
 
 Inductive Argument :=
-  | Arg : Id -> Argument.
+  | Arg : id -> Argument.
 
 Inductive Assignment :=
-  | Assgnmt : Id -> Id -> Assignment.
+  | Assgnmt : id -> id -> Assignment.
 
 Inductive FormalArg :=
-  | FArg : ClassName -> Id -> FormalArg.
+  | FArg : ClassName -> id -> FormalArg.
 
 Inductive Constructor :=
-  | KDecl : Id -> [FormalArg] -> [Argument] -> [Assignment] -> Constructor.
+  | KDecl : id -> [FormalArg] -> [Argument] -> [Assignment] -> Constructor.
 
 Inductive FieldDecl :=
-  | FDecl : ClassName -> Id -> FieldDecl.
+  | FDecl : ClassName -> id -> FieldDecl.
 
-Inductive Exp :=
+Inductive Exp : Set :=
   | ExpVar : Var -> Exp
-  | ExpFieldAccess : Exp -> Id -> Exp
-  | ExpMethodInvoc: Exp -> Id -> [Exp] -> Exp
+  | ExpFieldAccess : Exp -> id -> Exp
+  | ExpMethodInvoc: Exp -> id -> [Exp] -> Exp
   | ExpCast : ClassName -> Exp -> Exp
-  | ExpNew : Id -> [Exp] -> Exp.
+  | ExpNew : id -> [Exp] -> Exp.
 
 Inductive MethodDecl :=
-  | MDecl : ClassName -> Id -> [FormalArg] -> Id -> MethodDecl.
+  | MDecl : ClassName -> id -> [FormalArg] -> id -> MethodDecl.
 
-Inductive ClassDecl :=
-  | CDecl: Id -> ClassName -> [FieldDecl] -> Constructor -> [MethodDecl] -> ClassDecl.
+Inductive ClassDecl:=
+  | CDecl: id -> ClassName -> [FieldDecl] -> Constructor -> [MethodDecl] -> ClassDecl.
 
 Inductive Program :=
   | CProgram : [ClassDecl] -> Exp -> Program.
 
-Parameter CT: [ClassDecl].
+Parameter CT: @partial_map ClassDecl.
 (*We will assume a global CT to make our definitions easier
  *To instance the CT use Hypothesis x: CT = ... *)
 
-Definition extends (C D : ClassName) : Prop :=
+Definition extends (C D : ClassName) :=
   match C with
-  | ClassObject => False
-  | ClassId cname =>
-    exists fdecls kons mdecl, List.In (CDecl cname D fdecls kons mdecl) CT
+  | ClassObject => None
+  | ClassId cname => find cname CT
   end.
+
+  Print extends.
 
 
 Reserved Notation "C '<:' D " (at level 40).
 
 Inductive Subtype : ClassName -> ClassName -> Set :=
-  | S_Refl: forall C:ClassName, C <: C
+  | S_Refl: forall C: ClassName, C <: C
   | S_Trans: forall (C D E: ClassName), 
-    C <: D -> D <: E -> C <: E
+    C <: D -> 
+    D <: E -> 
+    C <: E
   | S_Decl: forall C D, 
-    extends C D -> C <: D
+    (exists decl, extends C D = Some decl) -> 
+    C <: D
 where "C '<:' D" := (Subtype C D).
+
+Definition Bind := @partial_map Exp.
+
+
+Lemma eq_var_dec : forall (v v': Var), {v = v'} + {v <> v'}.
+Proof.
+  intros. destruct v, v'; try eauto.
+  Case "This VarId".
+    right; intro.
+    inversion H.
+  Case "VarId This".
+    right; intro; inversion H.
+  Case "VarId VarId".
+    destruct i, i0.
+    destruct eq_nat_dec with (n:=n) (m:=n0).
+    SCase "n = n0".
+      left; rewrite e; reflexivity.
+    SCase "n <> n0".
+      right; intro H.
+      inversion H. auto.
+Defined.
+
+Fixpoint subst (e: Exp) (v: Var) (v': Exp) :=
+  match e with
+  | ExpVar var => if eq_var_dec var v then v' else ExpVar var
+  | ExpFieldAccess exp i => ExpFieldAccess (subst exp v v') i
+  | ExpMethodInvoc exp i exps => 
+      ExpMethodInvoc (subst exp v v') i (map (fun x => subst x v v') exps)
+  | ExpCast cname exp => ExpCast cname (subst exp v v')
+  | ExpNew cname exps => ExpNew cname (map (fun x => subst x v v') exps)
+  end.
+
+Notation " '[' v ':=' v' ']' e " := (subst e v v') (at level 40).  
+
+Eval compute in ([ (VarId (Id 1)) := ExpFieldAccess (ExpVar This) (Id 2)] ExpVar (VarId (Id 1))).
 
